disk-betree/ImplModelDealloc.i.dfy
@@ -1,0 +1,112 @@
+include "ImplModelCache.i.dfy"
+
+module ImplModelDealloc { 
+  import opened ImplModel
+  import opened ImplModelIO
+  import opened ImplModelCache
+
+  import opened Options
+  import opened Maps
+  import opened Sequences
+  import opened Sets
+
+  import opened NativeTypes
+
+  predicate deallocable(s: Variables, ref: BT.G.Reference)
+  {
+    && s.Ready?
+    && ref in IIndirectionTable(s.ephemeralIndirectionTable).graph
+    && ref != BT.G.Root()
+    && forall r | r in IIndirectionTable(s.ephemeralIndirectionTable).graph :: ref !in IIndirectionTable(s.ephemeralIndirectionTable).graph[r]
+  }
+
+  function Dealloc(k: Constants, s: Variables, io: IO, ref: BT.G.Reference)
+  : (res : (Variables, IO))
+  requires Inv(k, s)
+  requires io.IOInit?
+  requires deallocable(s, ref)
+  {
+    if (
+      && s.frozenIndirectionTable.Some?
+      && ref in s.frozenIndirectionTable.value
+      && var entry := s.frozenIndirectionTable.value[ref];
+      && var (loc, _) := entry;
+      && loc.None?
+    ) then (
+      (s, io)
+    ) else if !BC.OutstandingBlockReadsDoesNotHaveRef(s.outstandingBlockReads, ref) then (
+      (s, io)
+    ) else (
+      var s' := s
+        .(ephemeralIndirectionTable := MapRemove1(s.ephemeralIndirectionTable, ref))
+        .(cache := MapRemove1(s.cache, ref));
+      (s', io)
+    )
+  }
+
+  lemma DeallocCorrect(k: Constants, s: Variables, io: IO, ref: BT.G.Reference)
+  requires Inv(k, s)
+  requires io.IOInit?
+  requires deallocable(s, ref)
+  ensures var (s', io') := Dealloc(k, s, io, ref);
+      && WFVars(s')
+      &&  M.Next(Ik(k), IVars(s), IVars(s'), UI.NoOp, diskOp(io'))
+  {
+    var (s', io') := Dealloc(k, s, io, ref);
+
+    if (
+      && s.frozenIndirectionTable.Some?
+      && ref in s.frozenIndirectionTable.value
+      && var entry := s.frozenIndirectionTable.value[ref];
+      && var (loc, _) := entry;
+      && loc.None?
+    ) {
+      assert noop(k, IVars(s), IVars(s'));
+      return;
+    }
+
+    if !BC.OutstandingBlockReadsDoesNotHaveRef(s.outstandingBlockReads, ref) {
+      assert noop(k, IVars(s), IVars(s'));
+      return;
+    }
+
+    var iDiskOp := M.IDiskOp(diskOp(io));
+    assert BC.Unalloc(Ik(k), IVars(s), IVars(s'), iDiskOp, ref);
+    assert BBC.BlockCacheMove(Ik(k), IVars(s), IVars(s'), UI.NoOp, iDiskOp, BC.UnallocStep(ref));
+    assert stepsBC(k, IVars(s), IVars(s'), UI.NoOp, io, BC.UnallocStep(ref));
+    // assert M.NextStep(Ik(k), IVars(s), IVars(s'), UI.NoOp, io.diskOp(), M.Step(BBC.BlockCacheMoveStep(BC.UnallocStep(ref))));
+  }
+
+  /*
+  method FindDeallocable(s: Variables) returns (ref: Option<Reference>)
+  requires WFVars(s)
+  requires s.Ready?
+  ensures ref.Some? ==> ref.value in IIndirectionTable(s.ephemeralIndirectionTable).graph
+  ensures ref.Some? ==> deallocable(s, ref.value)
+  ensures ref.None? ==> forall r | r in IIndirectionTable(s.ephemeralIndirectionTable).graph :: !deallocable(s, r)
+  {
+    // TODO once we have an lba freelist, rewrite this to avoid extracting a `map` from `s.ephemeralIndirectionTable`
+    var ephemeralTable := s.ephemeralIndirectionTable.ToMap();
+    var ephemeralRefs := SetToSeq(ephemeralTable.Keys);
+
+    assume |ephemeralRefs| < 0x1_0000_0000_0000_0000;
+
+    var i: uint64 := 0;
+    while i as int < |ephemeralRefs|
+    invariant i as int <= |ephemeralRefs|
+    invariant forall k : nat | k < i as nat :: (
+        && ephemeralRefs[k] in IIndirectionTable(s.ephemeralIndirectionTable).graph
+        && !deallocable(s, ephemeralRefs[k]))
+    {
+      var ref := ephemeralRefs[i];
+      var isDeallocable := Deallocable(s, ref);
+      if isDeallocable {
+        return Some(ref);
+      }
+      i := i + 1;
+    }
+    assert forall r | r in IIndirectionTable(s.ephemeralIndirectionTable).graph :: !deallocable(s, r);
+    return None;
+  }
+  */
+}
